comments

ulib/experimental/Steel.Hashtbl.fst
@@ -1,4 +1,23 @@
-module Steel.IArray
+(*
+   Copyright 2021 Microsoft Research
+
+   Licensed under the Apache License, Version 2.0 (the "License");
+   you may not use this file except in compliance with the License.
+   You may obtain a copy of the License at
+
+       http://www.apache.org/licenses/LICENSE-2.0
+
+   Unless required by applicable law or agreed to in writing, software
+   distributed under the License is distributed on an "AS IS" BASIS,
+   WITHOUT WARRANTIES OR CONDITIONS OF ANY KIND, either express or implied.
+   See the License for the specific language governing permissions and
+   limitations under the License.
+
+   Authors: Aseem Rastogi
+*)
+
+
+module Steel.Hashtbl
 
 open Steel.FractionalPermission
 open Steel.Memory
@@ -15,8 +34,19 @@ module A = Steel.Array
 
 #set-options "--ide_id_info_off --print_implicits"
 
+/// We implement the table using an array of length n as the store,
+///
+/// The elements of the array are (k, v) pairs in the hashtable
+///
+/// For a key k, we would compute the index in the array as ((h k) % store.len)
+///
+/// We will then lookup the index, if it is Some (k', _) then k' == k implies that the key k is present
+///   in the table
+///
+/// We also maintain a ghost reference to store the logical map view of the hashtable
+
 noeq
-type iarray k v (h:hash_fn_t k) = {
+type tbl k v (h:hash_fn k) = {
   store_len    : n:u32{U32.v n > 0};
   store        : A.array (option (k & v));
   g_repr       : ghost_ref (Map.t k v);
@@ -24,26 +54,44 @@ type iarray k v (h:hash_fn_t k) = {
   store_len_pf : squash (A.length store == U32.v store_len);
 }
 
-let seq_props (#k:eqtype) (#v:Type0) (h:hash_fn_t k)
-  (s:Seq.seq (option (k & v))) : prop =
-  
+
+/// The underlying sequence representation of the hashtable store has
+///   the following properties:
+///
+/// - Its length is bounded by u32
+/// - For a Some (k, _) entry at index i, (h k % len == i)
+
+let seq_props (#k:eqtype) (#v:Type0) (h:hash_fn k) (s:Seq.seq (option (k & v))) : prop =  
   0 < Seq.length s /\ UInt.size (Seq.length s) 32 /\
   
-  (forall (i:nat{i < Seq.length s}).
-     Some? (Seq.index s i) ==>
-     (let Some (x, _) = Seq.index s i in
-      U32.v (h x) `UInt.mod` (Seq.length s) == i))
+  (forall (i:nat{i < Seq.length s}). Some? (Seq.index s i) ==> (let Some (x, _) = Seq.index s i in
+                                                         U32.v (h x) `UInt.mod` Seq.length s == i))
 
-let seq_props_derived (#k:eqtype) (#v:Type0) (h:hash_fn_t k) (s:Seq.seq (option (k & v))) : prop =
+
+/// Given seq_props, we can prove that all the keys in the sequence are distinct
+///
+/// Sometimes in the proofs, it is easier to directly use the uniqueness property,
+///   rather than the seq_props
+
+let seq_keys_distinct (#k:eqtype) (#v:Type0) (s:Seq.seq (option (k & v))) : prop =
   forall (i j:(k:nat{k < Seq.length s})).{:pattern Seq.index s i; Seq.index s j}
     (i =!= j /\ Some? (Seq.index s i) /\ Some? (Seq.index s j)) ==>
-    (fst (Some?.v (Seq.index s i)) =!= fst (Some?.v (Seq.index s j)))  
+    (fst (Some?.v (Seq.index s i)) =!= fst (Some?.v (Seq.index s j)))
 
-let seq_props_derived_lemma (#k:eqtype) (#v:Type0) (h:hash_fn_t k) (s:Seq.seq (option (k & v)))
-  : Lemma
-      (requires seq_props h s)
-      (ensures seq_props_derived h s)
+
+/// We can easily prove the distinctness property given seq_props
+
+let seq_props_implies_seq_keys_distinct (#k:eqtype) (#v:Type0) (h:hash_fn k) (s:Seq.seq (option (k & v)))
+  : Lemma (requires seq_props h s) (ensures seq_keys_distinct s)
   = ()
+
+
+/// We now relate the store to the logical map
+///
+/// We first define a function to convert the sequence to a map
+///
+/// Later, we will maintain an invariant that the map obtained by applying this function
+///   to the store is a submap of the logical map
 
 let rec seq_to_map (#k:eqtype) (#v:Type0) (s:Seq.seq (option (k & v))) (default_v:v)
   : Tot (repr k v) (decreases Seq.length s)
@@ -52,16 +100,21 @@ let rec seq_to_map (#k:eqtype) (#v:Type0) (s:Seq.seq (option (k & v))) (default_
     else let hd, tl = Seq.head s, Seq.tail s in
          let m = seq_to_map tl default_v in
          match hd with
-         | Some (x, y) -> Map.upd m x y
          | None -> m
+         | Some (x, y) -> Map.upd m x y
 
 let submap_of (#k:eqtype) (#v:Type0) (m1 m2:Map.t k v) : prop =
   let open FStar.Map in
   forall (x:k). m1 `contains` x ==> (m2 `contains` x /\ m1 `sel` x == m2 `sel` x)
 
+
+/// The main separation logic assertion
+///
+/// Maintains the permission to the store and the ghost reference,
+///   and a pure proposition to relate the two
+
 [@@__reduce__]
-let store_contents_pred (#k:eqtype) (#v:Type0) (#h:hash_fn_t k)
-  (arr:iarray k v h) (m:repr k v)
+let store_contents_pred (#k:eqtype) (#v:Type0) (#h:hash_fn k) (arr:tbl k v h) (m:repr k v)
   : Seq.lseq (option (k & v)) (A.length arr.store) -> vprop
   = fun s ->
     A.varray_pts_to arr.store s
@@ -73,30 +126,148 @@ let store_contents_pred (#k:eqtype) (#v:Type0) (#h:hash_fn_t k)
 [@@__reduce__]
 let ipts_to arr m = h_exists (store_contents_pred arr m)
 
-let rec seq_to_map_empty_seq (#k:eqtype) (#v:Type0) (n:nat) (default_v:v)
+
+/// Some pure lemmas for a few properties of the store and logical map
+
+
+let rec seq_to_map_create (k:eqtype) (#v:Type0) (n:nat) (default_v:v)
   : Lemma (Map.equal (seq_to_map (Seq.create n None) default_v)
                      (empty_repr #k #v default_v))
   = if n = 0 then ()
     else begin
-      assert (Seq.equal (Seq.tail (Seq.create #(option (k & v)) n None))
-                        (Seq.create (n-1) None));
-      seq_to_map_empty_seq #k #v (n-1) default_v
+      assert (Seq.equal #(option (k & v)) (Seq.tail (Seq.create n None))
+                                          (Seq.create (n-1) None));
+      seq_to_map_create k (n-1) default_v
     end
 
-let rec seq_to_map_ith (#k:eqtype) (#v:Type0) (h:hash_fn_t k) (s:Seq.seq (option (k & v)))
-  (default_v:v)
+
+/// The ith entry in the sequence, if it is Some (x, y) then in the corresponding map x |-> v
+///
+/// Note that this needs that the keys in the sequence are distinct
+
+let rec seq_to_map_ith (#k:eqtype) (#v:Type0) (s:Seq.seq (option (k & v))) (default_v:v)
   (i:nat{i < Seq.length s})
   : Lemma
-      (requires seq_props_derived h s /\ Some? (Seq.index s i))
-      (ensures (let Some (x, y) = Seq.index s i in
-                Map.contains (seq_to_map s default_v) x /\
-                Map.sel (seq_to_map s default_v) x == y))
+      (requires
+        seq_keys_distinct s /\
+        Some? (Seq.index s i))
+      (ensures (let open Map in
+                let Some (x, y) = Seq.index s i in
+                let m = seq_to_map s default_v in
+                m `contains` x /\
+                m `sel` x == y))
       (decreases i)
-  = if i = 0 then () else seq_to_map_ith h (Seq.tail s) default_v (i-1)
+  = if i = 0 then () else seq_to_map_ith (Seq.tail s) default_v (i-1)
+
+
+/// The domain of the seq_to_map map is strictly the entries in the sequence
+
+let rec seq_to_map_domain (#k:eqtype) (#v:Type0) (s:Seq.seq (option (k & v))) (default_v:v) (x:k)
+  : Lemma
+      (ensures
+        seq_to_map s default_v `Map.contains` x ==>  //if x is in the seq_to_map map,
+        (exists (i:nat{i < Seq.length s}).
+           Some? (Seq.index s i) /\
+           fst (Some?.v (Seq.index s i)) == x))  //then it must be in the sequence
+      (decreases Seq.length s)
+  = if Seq.length s = 0 then ()
+    else seq_to_map_domain (Seq.tail s) default_v x
+
+
+/// Commutation of seq_to_map with Seq.upd
+///
+/// It requires that the keys distinctness property in the original and updated sequence
+
+let rec seq_to_map_upd (#k:eqtype) (#v:Type0) (s:Seq.seq (option (k & v))) (default_v:v)
+  (i:nat{i < Seq.length s})
+  (x:k) (y:v)
+  : Lemma
+      (requires
+        seq_keys_distinct s /\
+        seq_keys_distinct (Seq.upd s i (Some (x, y))))
+      (ensures
+        seq_to_map (Seq.upd s i (Some (x, y))) default_v `submap_of`
+        Map.upd (seq_to_map s default_v) x y)
+      (decreases i)
+  = let m = seq_to_map s default_v in
+    let s1 = Seq.upd s i (Some (x, y)) in
+    let m1 = seq_to_map s1 default_v in
+
+    //To prove: m1 `submap_of` Map.upd m x y
+
+    if i = 0 then begin
+      let m_tl = seq_to_map (Seq.tail s) default_v in
+      match Seq.head s with
+      | None ->
+        assert (m == m_tl);
+        assert (m1 == Map.upd m_tl x y);
+        assert (m1 == Map.upd m x y)  //and submap_of is reflexive
+      | Some (x', y') ->
+        assert (m == Map.upd m_tl x' y');
+        assert (m1 == Map.upd m_tl x y);
+        //
+        //We need to prove:
+        //  Map.upd m_tl x y `submap_of` Map.upd (Map.upd m_tl x' y') x y
+        //
+        //Note that this would not be the case if m_tl `Map.contains` x'
+        //  since if it is, then it could be the case that m_tl[x'] = y'',
+        //  whereas its mapping on the right hand side is y'
+        //
+        //But we are in luck, we can prove that x' \notin m_tl
+        //
+        //And we prove it by appealing to the fact that a key in the seq_to_map map
+        //  must be present in the sequence
+        //
+        //Conversely, if a key is not in the sequence, then it is not in the map
+        //
+        seq_to_map_domain (Seq.tail s) default_v x';
+        assert (m1 `submap_of` Map.upd m x y)
+    end
+    else begin
+      seq_to_map_upd (Seq.tail s) default_v (i-1) x y;
+      //Induction hypothesis
+      assert (seq_to_map (Seq.upd (Seq.tail s) (i-1) (Some (x, y))) default_v `submap_of`
+              Map.upd (seq_to_map (Seq.tail s) default_v) x y);
+      match Seq.head s with
+      | None ->
+        assert (m == seq_to_map (Seq.tail s) default_v);
+        assert (m1 == seq_to_map (Seq.upd (Seq.tail s) (i-1) (Some (x, y))) default_v);
+        assert (m1 `submap_of` Map.upd m x y)  //directly from Induction hypothesis
+      | Some (x', y') ->
+        assert (m == Map.upd (seq_to_map (Seq.tail s) default_v) x' y');
+        assert (m1 == Map.upd (seq_to_map (Seq.upd (Seq.tail s) (i-1) (Some (x, y))) default_v) x' y');
+        //
+        //Apply Map.upd (...) x' y' to both the sides of `submap_of` in the Induction hypothesis
+        //
+        assert (Map.upd (seq_to_map (Seq.upd (Seq.tail s) (i-1) (Some (x, y))) default_v) x' y' `submap_of`
+                Map.upd (Map.upd (seq_to_map (Seq.tail s) default_v) x y) x' y');
+        //
+        //i.e.
+        //
+        assert (m1 `submap_of` Map.upd (Map.upd (seq_to_map (Seq.tail s) default_v) x y) x' y');
+
+        //
+        //We want the right side to be Map.upd (Map.upd (seq_to_map (Seq.tail s) default_v) x' y') x y
+        //
+        //We get there by proving that x' =!= x, and then the two updates can be commuted
+        //
+        //To get that x' =!= x, we appeal to the fact that
+        //  in the updated sequence the keys are distinct and i =!= 0
+        //
+
+        assert (Seq.index (Seq.upd s i (Some (x, y))) 0 == Some (x', y'));
+        assert (Seq.index (Seq.upd s i (Some (x, y))) i == Some (x, y));
+        assert (x =!= x');
+        assert (Map.equal (Map.upd (Map.upd (seq_to_map (Seq.tail s) default_v) x y) x' y')
+                          (Map.upd (Map.upd (seq_to_map (Seq.tail s) default_v) x' y') x y))        
+    end
+
+
+/// The main stateful API
 
 let create #k #v h x n =
-  let store = A.malloc #(option (k & v)) None n in
-  let g_ref = ghost_alloc_pt (G.hide (empty_repr #k #v x)) in
+  let store = A.malloc None n in
+  let g_ref = ghost_alloc_pt (G.hide (empty_repr (G.reveal x))) in
   let arr = {
     store_len = n;
     store = store;
@@ -104,16 +275,16 @@ let create #k #v h x n =
     default_v = x;
     store_len_pf = () } in
   let s = A.intro_varray_pts_to arr.store in
-  seq_to_map_empty_seq #k #v (U32.v n) x;
-  intro_pure (seq_props h s /\ submap_of (seq_to_map s arr.default_v) (empty_repr #k #v x));
-  assert_spinoff (ghost_pts_to g_ref full_perm (empty_repr #k #v x) ==
-                  ghost_pts_to arr.g_repr full_perm (empty_repr #k #v x));
-  change_equal_slprop (ghost_pts_to g_ref full_perm (empty_repr #k #v x))
-                      (ghost_pts_to arr.g_repr full_perm (empty_repr #k #v x));
-  intro_exists (G.reveal s) (store_contents_pred arr (empty_repr #k #v x));
+  seq_to_map_create k (U32.v n) (G.reveal x);
+  intro_pure (seq_props h s /\ submap_of (seq_to_map s arr.default_v) (empty_repr (G.reveal x)));
+  assert_spinoff (ghost_pts_to g_ref full_perm (empty_repr (G.reveal x)) ==
+                  ghost_pts_to arr.g_repr full_perm (empty_repr (G.reveal x)));
+  change_equal_slprop (ghost_pts_to g_ref full_perm (empty_repr (G.reveal x)))
+                      (ghost_pts_to arr.g_repr full_perm (empty_repr (G.reveal x)));
+  intro_exists (G.reveal s) (store_contents_pred arr (empty_repr (G.reveal x)));
   return arr
 
-let index #k #v #h #m a i =
+let get #k #v #h #m a i =
   let s = witness_exists () in
   A.elim_varray_pts_to a.store s;
   elim_pure (seq_props h s /\ seq_to_map s a.default_v `submap_of` m);
@@ -124,7 +295,7 @@ let index #k #v #h #m a i =
     | Some (i', v) ->
       if i = i'
       then begin
-        seq_to_map_ith h s a.default_v (U32.v (h i `U32.rem` a.store_len));
+        seq_to_map_ith s a.default_v (U32.v (h i `U32.rem` a.store_len));
         return (Some v)
       end
       else return None in
@@ -134,60 +305,21 @@ let index #k #v #h #m a i =
   intro_pure (Some? r ==> r == Some (Map.sel m i));
   return r
 
-let rec seq_to_map_domain (#k:eqtype) (#v:Type0) (s:Seq.seq (option (k & v))) (default_v:v) (x:k)
-  : Lemma
-      (ensures
-        seq_to_map s default_v `Map.contains` x ==>
-        (exists (i:nat{i < Seq.length s}). Some? (Seq.index s i) /\ fst (Some?.v (Seq.index s i)) == x))
-      (decreases Seq.length s)
-  = if Seq.length s = 0 then ()
-    else seq_to_map_domain (Seq.tail s) default_v x
-
-let rec seq_to_map_upd_aux (#k:eqtype) (#v:Type0) h (s:Seq.seq (option (k & v))) (default_v:v)
-  (i:nat{i < Seq.length s}) (x:k) (y:v)
-  : Lemma
-      (requires
-        seq_props_derived h s /\
-        seq_props_derived h (Seq.upd s i (Some (x, y))))
-      (ensures
-        seq_to_map (Seq.upd s i (Some (x, y))) default_v `submap_of`
-        Map.upd (seq_to_map s default_v) x y)
-      (decreases i)
-  = if i = 0 then begin
-      match Seq.head s with
-      | None -> ()
-      | Some (x', _) -> seq_to_map_domain (Seq.tail s) default_v x'
-    end
-    else begin
-      seq_to_map_upd_aux h (Seq.tail s) default_v (i-1) x y;
-      match Seq.head s with
-      | None -> ()
-      | Some (x', y') ->
-        assert (Seq.index (Seq.upd s i (Some (x, y))) 0 == Some (x', y'));
-        assert (Seq.index (Seq.upd s i (Some (x, y))) i == Some (x, y));
-        assert (x =!= x')
-    end
-
-let seq_to_map_upd (#k:eqtype) (#v:Type0) h (s:Seq.seq (option (k & v))) (default_v:v)
-  (m:Map.t k v)
-  (i:nat{i < Seq.length s}) (x:k) (y:v)
-  : Lemma
-      (requires
-        seq_props_derived h s /\
-        seq_props_derived h (Seq.upd s i (Some (x, y))) /\
-        seq_to_map s default_v `submap_of` m)
-      (ensures
-        seq_to_map (Seq.upd s i (Some (x, y))) default_v `submap_of` Map.upd m x y)
-  = seq_to_map_upd_aux h s default_v i x y
-            
-let upd #k #v #h #m a i x =
+let put #k #v #h #m a i x =
   let s = witness_exists () in
   A.elim_varray_pts_to a.store s;
   elim_pure (seq_props h s /\ seq_to_map s a.default_v `submap_of` m);
   A.upd a.store (h i `U32.rem` a.store_len) (Some (i, x));
   ghost_write_pt a.g_repr (Map.upd m i x);
   assert (seq_props #k #v h (Seq.upd s (U32.v (h i `U32.rem` a.store_len)) (Some (i, x))));
-  seq_to_map_upd #k #v h s a.default_v m (U32.v (h i `U32.rem` a.store_len)) i x;
+  seq_to_map_upd #k #v s a.default_v (U32.v (h i `U32.rem` a.store_len)) i x;
   let s = A.intro_varray_pts_to a.store in
   intro_pure (seq_props h s /\ seq_to_map s a.default_v `submap_of` Map.upd m i x);
   intro_exists (G.reveal s) (store_contents_pred a (Map.upd m i x))
+
+let free #k #v #h #m a =
+  let s = witness_exists () in
+  A.elim_varray_pts_to a.store s;
+  ghost_free_pt a.g_repr;
+  A.free a.store;
+  elim_pure (seq_props h s /\ seq_to_map s a.default_v `submap_of` m)
